src/drf/ADRF_PF2.v
@@ -23,7 +23,7 @@ Require Import PromiseConsistent.
 Require Import APromiseConsistent.
 From PromisingLib Require Import Loc.
 
-Require Import PF.
+Require Import APF.
 Require Import Race.
 Require Import Behavior.
 Require Import SimMemory.
